%!Tex Root = ../main.tex
% ./Packete.tex
% ./Design.tex
% ./Deklarationen.tex
% ./Vorbereitung.tex
% ./Aufgabe1.tex
% ./Aufgabe3.tex
% ./Aufgabe4.tex
% ./Bonus.tex

\section{Aufgabe 2}

\setcounter{task}{1}

\begin{frame}[allowframebreaks]{Aufgabe 2}{Aussagenlogik}
\begin{requirementsnoinc}
  \begin{align*}
    x\ \vee y &:=\quad x+y-x\cdot y\\
    x\wedge y &:=\quad x\cdot y\\
    {\neg x}  &:={1-x}
  \end{align*}
  \begin{itemize}
    \item \alert{es gilt:} $x^{2}=x\cdot x=x$, da $x\in\{0,1\}$ oder wenn man auf den $\wedge$-Operator zurückführt: $x^{2}=x\cdot x=x\wedge x=x$
  \end{itemize}
\end{requirementsnoinc}

\definecolor{VeniceBlue}{rgb}{0.043,0.392,0.627}
% \definecolor{Concrete}{rgb}{0.949,0.949,0.949}
\definecolor{Concrete}{rgb}{1, 1, 1}
\definecolor{TropicalBlue}{rgb}{0.807,0.917,0.976}

\begin{solutionnoinc}
\begin{table}
\centering
\begin{tblr}{
  cells = {Concrete,c},
  row{1} = {VeniceBlue,fg=white},
  cell{2}{5} = {TropicalBlue},
  cell{2}{7} = {TropicalBlue},
  cell{3}{5} = {TropicalBlue},
  cell{3}{7} = {TropicalBlue},
  cell{4}{5} = {TropicalBlue},
  cell{4}{7} = {TropicalBlue},
  cell{5}{5} = {TropicalBlue},
  cell{5}{7} = {TropicalBlue},
  cell{6}{5} = {TropicalBlue},
  cell{6}{7} = {TropicalBlue},
  cell{7}{5} = {TropicalBlue},
  cell{7}{7} = {TropicalBlue},
  cell{8}{5} = {TropicalBlue},
  cell{8}{7} = {TropicalBlue},
  cell{9}{5} = {TropicalBlue},
  cell{9}{7} = {TropicalBlue},
}
$x$ & $y$ & $z$ & $x\wedge y$ & $(x\wedge y) \wedge z$ & $y\wedge z$ & $(x\wedge y) \wedge z$ \\
 0  &  0  &  0  &     0       &            0           &      0      &           0            \\
 0  &  0  &  1  &     0       &            0           &      0      &           0            \\
 0  &  1  &  0  &     0       &            0           &      0      &           0            \\
 0  &  1  &  1  &     0       &            0           &      0      &           0            \\
 1  &  0  &  0  &     0       &            0           &      0      &           0            \\
 1  &  0  &  1  &     0       &            0           &      0      &           0            \\
 1  &  1  &  0  &     1       &            0           &      0      &           0            \\
 1  &  1  &  1  &     1       &            1           &      1      &           1            
\end{tblr}
\end{table}
\end{solutionnoinc}

\begin{solutionnoinc}
\begin{table}
\centering
\begin{tblr}{
  cells = {Concrete,c},
  row{1} = {VeniceBlue,fg=white},
  cell{2}{5} = {TropicalBlue},
  cell{2}{7} = {TropicalBlue},
  cell{3}{5} = {TropicalBlue},
  cell{3}{7} = {TropicalBlue},
  cell{4}{5} = {TropicalBlue},
  cell{4}{7} = {TropicalBlue},
  cell{5}{5} = {TropicalBlue},
  cell{5}{7} = {TropicalBlue},
  cell{6}{5} = {TropicalBlue},
  cell{6}{7} = {TropicalBlue},
  cell{7}{5} = {TropicalBlue},
  cell{7}{7} = {TropicalBlue},
  cell{8}{5} = {TropicalBlue},
  cell{8}{7} = {TropicalBlue},
  cell{9}{5} = {TropicalBlue},
  cell{9}{7} = {TropicalBlue},
}
$x$ & $y$ & $z$ & $x\vee y$ & $(x\vee y) \vee z$ & $y\vee z$ & $(x\vee y) \vee z$ \\
0   & 0   & 0   & 0           & 0                      & 0           & 0                      \\
0   & 0   & 1   & 0           & 1                      & 1           & 1                      \\
0   & 1   & 0   & 1           & 1                      & 1           & 1                      \\
0   & 1   & 1   & 1           & 1                      & 1           & 1                      \\
1   & 0   & 0   & 1           & 1                      & 0           & 1                      \\
1   & 0   & 1   & 1           & 1                      & 1           & 1                      \\
1   & 1   & 0   & 1           & 1                      & 1           & 1                      \\
1   & 1   & 1   & 1           & 1                      & 1           & 1
\end{tblr}
\end{table}
\end{solutionnoinc}

\begin{solution}
\begin{table}
\centering
\begin{tblr}{
  cells = {Concrete,c},
  row{1} = {VeniceBlue,fg=white},
  cell{2}{4} = {TropicalBlue},
  cell{2}{6} = {TropicalBlue},
  cell{3}{4} = {TropicalBlue},
  cell{3}{6} = {TropicalBlue},
  cell{4}{4} = {TropicalBlue},
  cell{4}{6} = {TropicalBlue},
  cell{5}{4} = {TropicalBlue},
  cell{5}{6} = {TropicalBlue},
}
$x$ & $y$ & $y\wedge \neg y$ & $x\vee(y\wedge \neg y)$ & $y\vee \neg y$ & $x \wedge (y\vee \neg y)$ \\
0   & 0   & 0                & 0                       & 1              & 0                         \\
0   & 1   & 0                & 0                       & 1              & 0                         \\
1   & 0   & 0                & 1                       & 1              & 1                         \\
1   & 1   & 0                & 1                       & 1              & 1                         
\end{tblr}
\end{table}
\end{solution}
\end{frame}

\begin{frame}[allowframebreaks]{Aufgabe 2}{Aussagenlogik}
  \begin{solutionnoinc}
    \begin{align*}
      x\,\vee\,\left(x\wedge y\right)&=x+(x\cdot y)-x(x\cdot y)\\ 
      &{=x+x y-x^{2}y}\\ 
      &{\overset{*}{=}x+x y-x y}\\ 
      &{=x}
    \end{align*}
  \end{solutionnoinc}
  \begin{solutionnoinc}
    \begin{align*}
      x\wedge(x\vee y)&=x\cdot(x+y-x y)\\ 
      &=x^{2}+x y-x^{2}y\\ 
      &\overset{*}{=}x+x y-x y\\ 
      &=x
    \end{align*}
  \end{solutionnoinc}
  \begin{solutionnoinc}    
    \begin{align*}
      (x\vee y)\land(x\vee z)&=(x+y-x y)\cdot(x+z-x z)\\
      &=x(x+z-xz)+y(x+z-xz)+xy(x+z - x z)\\
      &=x^2+xz-x^2z+xy+yz-xyz-x^2y-xyz+x^2yz\\
      &=x+xz-x^2z+xy+yz-xyz-xy-xyz+xyz\\
      &=x+yz-xyz\\
      &=x+(y\wedge z)-x\wedge(y\wedge z)\\
      &=x\vee(y\wedge z)
    \end{align*}
  \end{solutionnoinc}
  \begin{solution}
    \begin{align*}
      (x\wedge y)\vee(x\wedge z)&=x y+x z-(x y\cdot x z)\\ 
      &{{}=x y+x z-(x^{2}y z)}\\ 
      &{{}=x y+x z-(x y z)}\\ 
      &{{}=x(y+z - yz)}\\ 
      &=x \cdot (y\vee z)\\
      &=x \wedge(y\vee z)
    \end{align*}
  \end{solution}
\end{frame}
