%!Tex Root = ../main.tex
% ./Packete.tex
% ./Design.tex
% ./Deklarationen.tex
% ./Vorbereitung.tex
% ./Aufgabe2.tex
% ./Aufgabe3.tex
% ./Aufgabe4.tex
% ./Bonus.tex

\section{Aufgabe 1}

\setcounter{task}{1}

\begin{frame}[allowframebreaks]{Aufgabe 1}{Vollst√§ndige Induktion}
  \begin{requirementsnoinc}
    \begin{itemize}
      \item $\displaystyle\sum_{i=0}^{n}z^{i}={\frac{z^{n+1}-1}{z-1}}$
      \item \alert{es gelte:} $\displaystyle z\in\mathbb{R}\setminus\{1\}\ \mathrm{und}\ n\in\mathbb{N}$
    \end{itemize}
  \end{requirementsnoinc}
  \begin{solutionnoinc}
    \begin{itemize}
      \item \alert{Induktionsanfang:} $n=0$
        \[
          \sum_{i=0}^{0}z^{i}=1 = \frac{z-1}{z-1}=\frac{z^{0+1}-1}{z-1} 
        \]
      \item \alert{Induktionsschritt:} $n \to n+1$
        \begin{align*}
          \sum_{i=0}^{n+1}z^{i}&=(\sum_{i=0}^{n}z^{i})+z^{n+1}\\
                               &= \frac{z^{n+1}-1}{z-1}+z^{n+1}\quad\mathrm{wegen~Induktionsvoraussetzung}\\
                               &= \frac{z^{n+1}-1+z^{n+1}\cdot(z-1)}{z-1}\\
                               &= \frac{z^{n+1}-1+z^{n+2}-z^{n+1}}{z-1}\\
                               &= \frac{z^{n+2}-1}{z-1}
        \end{align*}
    \end{itemize}
  \end{solutionnoinc}
\end{frame}
