%!Tex Root = ../main.tex
% ./Packete.tex
% ./Design.tex
% ./Deklarationen.tex
% ./Vorbereitung.tex
% ./Aufgabe1.tex
% ./Aufgabe3.tex
% ./Aufgabe4.tex
% ./Appendix.tex

\section{Aufgabe 2}

\setcounter{exercise}{1}

\begin{frame}{Aufgabe \thesection}{n-Bit Inkrementer $INC_n$}
  \begin{solutionnoinc}
    \includegraphics[height=0.6\paperheight, center]{figures/incrementer.png}
  \end{solutionnoinc}
\end{frame} 

\begin{frame}{Aufgabe \thesection}{n-Bit Inkrementer $INC_n$}
  \begin{solution}
    \centering
    \input{./content/ex2_8}
  \end{solution}
\end{frame} 

\begin{frame}{Aufgabe \thesection}{n-Bit Inkrementer $INC_n$}
  \begin{solution}
    \begin{itemize}
      \setlength{\itemsep}{0cm}
      \setlength{\parsep}{0cm}
      \setlength{\parskip}{0.2cm}
      \item \alert{Tiefe:}
      \begin{itemize}
        \item \alert{$k=0$:} $1$ 
        \item \alert{$k=1$:} $1 + 3\cdot 1 = 4$ 
        \item \alert{$k=2$:} $1 + 3\cdot 2 = 7$ 
        \item \alert{$k=3$:} $1 + 3\cdot 3 = 10$ 
        \item \alert{allgemein:} 
        \begin{itemize}
          \item $\mathrm{depth}(\mathrm{CSA-INC}_{\frac{n}{2^k} }) = \mathrm{depth}(\mathrm{CSA-INC}_{1}) = \mathrm{depth}(\mathrm{HA}) = 1$
          \item $\mathrm{depth}(\mathrm{CSA-INC}_{n}) = \mathrm{depth}(\mathrm{CSA-INC}_{\frac{n}{2^1}}) + \mathrm{depth}(\mathrm{MUX_{\frac{n}{2}+1}}) = \mathrm{depth}(\mathrm{CSA-INC}_{\frac{n}{2^1}}) + 3 = \mathrm{depth}(\mathrm{CSA-INC}_{\frac{n}{2^2}}) + 3 + 3 = \mathrm{depth}(\mathrm{CSA-INC}_{\frac{n}{2^k}}) + 3 \cdot k = 3\cdot k + 1= 3\cdot log(n) + 1$
        \end{itemize}
      \end{itemize}
    \end{itemize}
  \end{solution}
  % \framebreak
\end{frame}

\begin{frame}{Aufgabe \thesection}{n-Bit Inkrementer $INC_n$}
  \begin{solution}
    \begin{itemize}
      \setlength{\itemsep}{0cm}
      \setlength{\parsep}{0cm}
      \setlength{\parskip}{0.2cm}
      \item \alert{Kosten:}
      \begin{itemize}
        \item \alert{$k=0$:} $2$ 
        \item \alert{$k=1$:} $2 \cdot 2 + (3\cdot1+2)\cdot 1 = 9$ 
        \item \alert{$k=2$:} $2 \cdot 4 + (3\cdot1+2)\cdot 2 + (3\cdot2+2)\cdot 1 = 26$ 
        \item \alert{$k=3$:} $2 \cdot 8 + (3\cdot1+2)\cdot 4 + (3\cdot2+2)\cdot 2 + (3\cdot4+2)\cdot 1 = 66$ 
        \item \alert{allgemein:}
        \begin{itemize}
          \item $\mathrm{cost}(\mathrm{CSA-INC}_{\frac{n}{2^k} }) = \mathrm{cost}(\mathrm{CSA-INC}_{1}) = \mathrm{cost}(\mathrm{HA}) = 2$
          \item $\displaystyle\mathrm{cost}(\mathrm{CSA-INC}_{n}) 
            = 2\cdot\mathrm{cost}(\mathrm{CSA-INC}_{\frac{n}{2^1}}) + \mathrm{cost}(\mathrm{MUX}_{\frac{n}{2^1}+1}) 
            = 2\cdot\mathrm{cost}(\mathrm{CSA-INC}_{\frac{n}{2^1}}) + (3 \cdot 2^{k-1} + 2) \cdot 1
            = 2 \cdot 2 \cdot\mathrm{cost}(\mathrm{CSA-INC}_{\frac{n}{2^2}}) + (3 \cdot 2^{k-2} + 2) \cdot 2 + (3 \cdot 2^{k-1} + 2) \cdot 1
            = 2^k \cdot\mathrm{cost}(\mathrm{CSA-INC}_{\frac{n}{2^k}}) + (3 \cdot 2^{0} + 2) \cdot 2^{k-1} + (3 \cdot 2^{1} + 2) \cdot 2^{k-2} + \ldots + (3 \cdot 2^{k-2} + 2) \cdot 2^1 + (3 \cdot 2^{k-1} + 2) \cdot 2^0 
            %= n \cdot 2 + (3 \cdot 2^{0} + 2) \cdot \frac{n}{2} + (3 \cdot 2^{1} + 2) \cdot \frac{n}{2^2} + \ldots + (3 \cdot \frac{n}{2} + 2) \cdot \frac{n}{2^k}
            = n \cdot 2 + \sum_{i=0}^{k-1} (3 \cdot 2^{k-i-1} + 2) \cdot 2^i
            = n \cdot 2 + \sum_{i=0}^{log(n)-1} (3 \cdot 2^{log(n)-i-1} + 2) \cdot 2^i = 4n + 3n \cdot \frac{log(n)}{2} - 2$
            % 2n + 2n + 3n \cdot \frac{log(n)}{2} - 2 
        \end{itemize}
      \end{itemize}
    \end{itemize}
  \end{solution}
\end{frame}
