%!Tex Root = ../main.tex
% ./Packete.tex
% ./Design.tex
% ./Deklarationen.tex
% ./Vorbereitung.tex
% ./Aufgabe1.tex
% ./Aufgabe2.tex
% ./Aufgabe4.tex
% ./Appendix.tex

\section{Aufgabe 3}

\setcounter{exercise}{1}

\begin{frame}[allowframebreaks]{Aufgabe \thesection}{Signextension}
  \begin{solutionnoinc}
    \begin{enumerate}
      \item \alert{Zurückführung auf Sign Extension um $1$ Bit:}\\
        \tiny 
        \alert{Lemma:} Sei $a\in\mathbb{B}^n, a = a_{n-1}\ldots a_0$. Dann gilt $[a]_2 = [a_{n-1}a]_2$.\\
        Beweis:\\
        $\displaystyle[a_{n-1}a]_{2}=-a_{n-1}\cdot2^{n}+\sum_{i=0}^{n-i}a_{i}\cdot2^{i}=-a_{n-1}\cdot2^{n}+\left(a_{n-1}\cdot2^{n-1}+\sum_{i=0}^{n-2}a_{i}\cdot2^{i}\right)=-a_{n-1}\cdot2^{n-1}+\sum_{i=0}^{n-2}a_{i}\cdot2^{i}=\left[a\right]_2$\\
        Damit: $[y]_{2}=[y_{n-1}^{1}y]_{2}=[y_{n-1}^{2}y_{n-1}^{1}y]_{2}=\cdot\cdot\cdot=[y_{n-1}^{k}\ldots y_{n-1}^{1}y]_{2}=[\mathrm{sext_{k}}(y)]_{2}.$
    \end{enumerate}
  \end{solutionnoinc}
  \begin{solution}
    \begin{enumerate}
      \item[2.] \alert{Direkter Beweis:}
        \tiny
        Sei $y\in\mathbb{B}^n, y=y_{n-1}\ldots y_0$

        $\begin{aligned}
          {\left[\operatorname{sext}_{\mathrm{k}}(y)\right]_2=[\underbrace{y_{n-1} \ldots y_{n-1}}_{k-m a l}y]_2 } & =\sum_{i=0}^{n-2} y_i \cdot 2^i+\sum_{i=n-1}^{n+k-2} y_{n-1} \cdot 2^i-y_{n-1} \cdot 2^{n+k-1} \\
                                                                                                                   & =\sum_{i=0}^{n-2} y_i \cdot 2^i+y_{n-1} \cdot\left(\sum_{i=0}^{n+k-2} 2^i-\sum_{i=0}^{n-2} 2^i\right)-y_{n-1} \cdot 2^{n+k-1} \\
                                                                                                                   & =\sum_{i=0}^{n-2} y_i \cdot 2^i+y_{n-1} \cdot\left(\frac{2^{n+k-1}-1}{2-1}-\frac{2^{n-1}-1}{2-1}\right)-y_{n-1} \cdot 2^{n+k-1} \\
                                                                                                                   & =\sum_{i=0}^{n-2} y_i \cdot 2^i+y_{n-1} \cdot 2^{n+k-1}-y_{n-1} \cdot 2^{n-1}-y_{n-1} \cdot 2^{n+k-1} \\
                                                                                                                   & =\sum_{i=0}^{n-2} y_i \cdot 2^i-y_{n-1} \cdot 2^{n-1} \\
                                                                                                                   & =[y]_2
        \end{aligned}$
    \end{enumerate}
  \end{solution}
\end{frame}
